\documentclass{article}

\usepackage{amsmath}

\begin{document}
\section{Gradient Descent}


\begin{align}
  % Po formuli odvoda vemo:
  C' = \lim_{\epsilon \to 0}\frac{C(w_i + \epsilon) - C(w_i)}{\epsilon}
\end{align}

\subsection{``Twice''}
\begin{align}
    C(w) &= \frac{1}{n}{\sum_{i=1}^{n}(x_iw - y_i)^2} \\
    % Poiscemo odvod C(w)
    C'(w) &= \frac{1}{n}{\sum_{i=1}^{n}(x_iw - y_i)^2} \\
          &= \left(\frac{1}{n}{\sum_{i=1}^{n}(x_iw - y_i)^2}\right)'= \\
          &= \frac{1}{n}\left(\sum_{i=1}^{n}(x_iw - y_i)^2\right)'  = \\
          &= \frac{1}{n}\sum_{i=1}^{n}\left((x_iw - y_i)^2\right)'  = \\
          % y_i   - is a constant that is going to be equal to 0 => we can remove it
          % x_i*w - w is a constant (1) so we can remove it and we are left with x_i
          &= \frac{1}{n}\sum_{i=1}^{n}2(x_iw - y_i)x_i  = \\
          &= \frac{1}{n}\sum_{i=1}^{n}2(x_iw - y_i)x_i  = \\
\end{align}
\begin{align}
  C(w)  &= \frac{1}{n}{\sum_{i=1}^{n}(x_iw - y_i)^2} \\
  C'(w) &= \frac{1}{n}\sum_{i=1}^{n}2(x_iw - y_i)x_i  \\
\end{align}

\end{document}